# computational-logic-homework-3-solved
**TO GET THIS SOLUTION VISIT:** [COMPUTATIONAL-LOGIC Homework 3 Solved](https://www.ankitcodinghub.com/product/computational-logic-homework-3-solved/)


---

ðŸ“© **If you need this solution or have special requests:** **Email:** ankitcoding@gmail.com  
ðŸ“± **WhatsApp:** +1 419 877 7882  
ðŸ“„ **Get a quote instantly using this form:** [Ask Homework Questions](https://www.ankitcodinghub.com/services/ask-homework-questions/)

*We deliver fast, professional, and affordable academic help.*

---

<h2>Description</h2>



<div class="kk-star-ratings kksr-auto kksr-align-center kksr-valign-top" data-payload="{&quot;align&quot;:&quot;center&quot;,&quot;id&quot;:&quot;93371&quot;,&quot;slug&quot;:&quot;default&quot;,&quot;valign&quot;:&quot;top&quot;,&quot;ignore&quot;:&quot;&quot;,&quot;reference&quot;:&quot;auto&quot;,&quot;class&quot;:&quot;&quot;,&quot;count&quot;:&quot;0&quot;,&quot;legendonly&quot;:&quot;&quot;,&quot;readonly&quot;:&quot;&quot;,&quot;score&quot;:&quot;0&quot;,&quot;starsonly&quot;:&quot;&quot;,&quot;best&quot;:&quot;5&quot;,&quot;gap&quot;:&quot;4&quot;,&quot;greet&quot;:&quot;Rate this product&quot;,&quot;legend&quot;:&quot;0\/5 - (0 votes)&quot;,&quot;size&quot;:&quot;24&quot;,&quot;title&quot;:&quot;COMPUTATIONAL-LOGIC Homework 3 Solved&quot;,&quot;width&quot;:&quot;0&quot;,&quot;_legend&quot;:&quot;{score}\/{best} - ({count} {votes})&quot;,&quot;font_factor&quot;:&quot;1.25&quot;}">

<div class="kksr-stars">

<div class="kksr-stars-inactive">
            <div class="kksr-star" data-star="1" style="padding-right: 4px">


<div class="kksr-icon" style="width: 24px; height: 24px;"></div>
        </div>
            <div class="kksr-star" data-star="2" style="padding-right: 4px">


<div class="kksr-icon" style="width: 24px; height: 24px;"></div>
        </div>
            <div class="kksr-star" data-star="3" style="padding-right: 4px">


<div class="kksr-icon" style="width: 24px; height: 24px;"></div>
        </div>
            <div class="kksr-star" data-star="4" style="padding-right: 4px">


<div class="kksr-icon" style="width: 24px; height: 24px;"></div>
        </div>
            <div class="kksr-star" data-star="5" style="padding-right: 4px">


<div class="kksr-icon" style="width: 24px; height: 24px;"></div>
        </div>
    </div>

<div class="kksr-stars-active" style="width: 0px;">
            <div class="kksr-star" style="padding-right: 4px">


<div class="kksr-icon" style="width: 24px; height: 24px;"></div>
        </div>
            <div class="kksr-star" style="padding-right: 4px">


<div class="kksr-icon" style="width: 24px; height: 24px;"></div>
        </div>
            <div class="kksr-star" style="padding-right: 4px">


<div class="kksr-icon" style="width: 24px; height: 24px;"></div>
        </div>
            <div class="kksr-star" style="padding-right: 4px">


<div class="kksr-icon" style="width: 24px; height: 24px;"></div>
        </div>
            <div class="kksr-star" style="padding-right: 4px">


<div class="kksr-icon" style="width: 24px; height: 24px;"></div>
        </div>
    </div>
</div>


<div class="kksr-legend" style="font-size: 19.2px;">
            <span class="kksr-muted">Rate this product</span>
    </div>
    </div>
Let <em>S </em>be a binary predicate symbol, <em>P </em>and <em>Q </em>unary predicate symbols.

<ul>
<li>Find a natural deduction proof to show</li>
</ul>
âˆƒ<em>x</em>âˆƒ<em>y</em>(<em>S</em>(<em>x,y</em>) âˆ¨ <em>S</em>(<em>y,x</em>)) ` âˆƒ<em>x</em>âˆƒ<em>yS</em>(<em>x,y</em>)<em>.</em>

<ul>
<li>Find a natural deduction proof to show</li>
</ul>
âˆ€<em>x</em>âˆ€<em>y</em>âˆ€<em>z</em>(<em>S</em>(<em>x,y</em>)âˆ§<em>S</em>(<em>y,z</em>) =â‡’ <em>S</em>(<em>x,z</em>))<em>,</em>âˆ€<em>x</em>Â¬<em>S</em>(<em>x,x</em>) ` âˆ€<em>x</em>âˆ€<em>y</em>(<em>S</em>(<em>x,y</em>) =â‡’ Â¬<em>S</em>(<em>y,x</em>))<em>.</em>

<ul>
<li>Find a natural deduction proof to show</li>
</ul>
âˆƒ<em>x</em>âˆƒ<em>y</em>(<em>S</em>(<em>x,y</em>) âˆ¨ <em>S</em>(<em>y,x</em>))<em>,</em>Â¬âˆƒ<em>xS</em>(<em>x,x</em>) ` âˆƒ<em>x</em>âˆƒ<em>y</em>Â¬(<em>x </em>= <em>y</em>)<em>.</em>

<ul>
<li>Show that there is no natural deduction proof for âˆ€<em>x</em>(<em>P</em>(<em>x</em>) âˆ¨ <em>Q</em>(<em>x</em>)) ` âˆ€<em>xP</em>(<em>x</em>) âˆ¨ âˆ€<em>xQ</em>(<em>x</em>)<em>.</em></li>
<li>Semantically show</li>
</ul>
âˆ€<em>x</em>Â¬<em>Ï† </em>|= Â¬âˆƒ<em>xÏ†.</em>

1
